@prefix xsd: <http://www.w3.org/2001/XMLSchema#> .
@prefix owl: <http://www.w3.org/2002/07/owl#> .
@prefix : <http://www.wf4ever-project.org/vocab/wf#> .
@prefix xml: <http://www.w3.org/XML/1998/namespace> .
@prefix rdf: <http://www.w3.org/1999/02/22-rdf-syntax-ns#> .
@prefix rdfs: <http://www.w3.org/2000/01/rdf-schema#> .
@prefix skos: <http://www.w3.org/2004/02/skos/core#> .
@base <http://www.wf4ever-project.org/vocab/wf> .

<http://www.wf4ever-project.org/vocab/wf> rdf:type owl:Ontology ;
                                          
                                          rdfs:comment """This ontology describes an abstract workflow structure, which on the top level is defined as a WorkflowTemplate.

A WorkflowTemplate contains several ProcessTemplates, associated using the hasProcessTemplate property. Each of these (and the workflow template itself) hasInput and hasOutput some Parameter Input or Output. An ArtifactTempalte is associated with a Parameter using hasArtifactTemplate. The WorkflowTemplate also hasDataLink several DataLinks which forms the connection between parameters.

Thus this ontology allows the description a direct acyclic graph, or a dataflow. 

This ontology is meant as an upper ontology for more specific workflow definitions, and as a way to express abstract workflows. The wfprov ontology shows how to link these templates to an OPMV provenance trace of a workflow execution."""@en .


#################################################################
#
#    Annotation properties
#
#################################################################


rdfs:comment rdf:type owl:AnnotationProperty .





#################################################################
#
#    Datatypes
#
#################################################################




#################################################################
#
#    Object Properties
#
#################################################################


###  http://www.w3.org/2002/07/owl#topObjectProperty

owl:topObjectProperty rdf:type owl:ObjectProperty .



###  http://www.wf4ever-project.org/vocab/wf#hasArtifactTemplate

:hasArtifactTemplate rdf:type owl:ObjectProperty ;
                     
                     rdfs:comment "This property associates a process template parameter to the artifact template that characterizes it."@en ;
                     
                     rdfs:subPropertyOf owl:topObjectProperty ;
                     
                     rdfs:range :ArtifactTemplate ;
                     
                     rdfs:domain :Parameter .



###  http://www.wf4ever-project.org/vocab/wf#hasDataLink

:hasDataLink rdf:type owl:ObjectProperty ;
             
             rdfs:comment "This property is used to specify the data links of a given workflow template." ;
             
             rdfs:subPropertyOf owl:topObjectProperty ;
             
             rdfs:range :DataLink ;
             
             rdfs:domain :WorkflowTemplate .



###  http://www.wf4ever-project.org/vocab/wf#hasInput

:hasInput rdf:type owl:ObjectProperty ;
          
          rdfs:comment "This object property is used to specify the input parameter of a given process template."@en ;
          
          rdfs:range :Input ;
          
          rdfs:domain :ProcessTemplate .



###  http://www.wf4ever-project.org/vocab/wf#hasOutput

:hasOutput rdf:type owl:ObjectProperty ;
           
           rdfs:comment """This object property is used to specify the output parameter of a given process template.
"""@en ;
           
           rdfs:range :Output ;
           
           rdfs:domain :ProcessTemplate .



###  http://www.wf4ever-project.org/vocab/wf#hasProcessTemplate

:hasProcessTemplate rdf:type owl:ObjectProperty ;
                    
                    rdfs:comment "This object property is used to specify that the given workflow template contains the given process template as part of its definition."@en ;
                    
                    rdfs:range :ProcessTemplate ;
                    
                    rdfs:domain :WorkflowTemplate .



###  http://www.wf4ever-project.org/vocab/wf#hasSink

:hasSink rdf:type owl:ObjectProperty ;
         
         rdfs:comment "This property is used to specify the input parameter that acts as a sink to a given data link."@en ;
         
         rdfs:subPropertyOf owl:topObjectProperty ;
         
         rdfs:domain :DataLink ;
         
         rdfs:range :Input .



###  http://www.wf4ever-project.org/vocab/wf#hasSource

:hasSource rdf:type owl:ObjectProperty ;
           
           rdfs:comment "This property is used to specify the output parameter that acts as a source to a given data link."@en ;
           
           rdfs:subPropertyOf owl:topObjectProperty ;
           
           rdfs:domain :DataLink ;
           
           rdfs:range :Output .



###  http://www.wf4ever-project.org/vocab/wf#hasSubWorkflowTemplate

:hasSubWorkflowTemplate rdf:type owl:ObjectProperty ;
                        
                        rdfs:comment """This object property is used to associate a workflow template to another workflow template, specifying that the given workflow has the given sub-workflow as a contained process. 

This is a specialisation of hasProcessTemplate."""@en ;
                        
                        rdfs:range :WorkflowTemplate ;
                        
                        rdfs:domain :WorkflowTemplate ;
                        
                        rdfs:subPropertyOf :hasProcessTemplate .





#################################################################
#
#    Classes
#
#################################################################


###  http://www.wf4ever-project.org/vocab/wf#ArtifactTemplate

:ArtifactTemplate rdf:type owl:Class ;
                  
                  rdfs:comment """ArtifactTemplate is used to provide information about a class of artifacts. For example, it can be used to specify the datatype of a dataset or the structure of a document.

An ArtifactTemplate is associated with a Parameter using hasArtifactTemplate."""@en .



###  http://www.wf4ever-project.org/vocab/wf#DataLink

:DataLink rdf:type owl:Class ;
          
          rdfs:comment "DataLink is used to represent data dependencies between process templates"@en .



###  http://www.wf4ever-project.org/vocab/wf#Input

:Input rdf:type owl:Class ;
       
       rdfs:subClassOf :Parameter ;
       
       rdfs:comment "It represents input parameter of a process template"@en .



###  http://www.wf4ever-project.org/vocab/wf#Output

:Output rdf:type owl:Class ;
        
        rdfs:subClassOf :Parameter ;
        
        rdfs:comment "Represents output parameter of a process template"@en .



###  http://www.wf4ever-project.org/vocab/wf#Parameter

:Parameter rdf:type owl:Class ;
           
           owl:equivalentClass [ rdf:type owl:Class ;
                                 owl:unionOf ( :Input
                                               :Output
                                             )
                               ] ;
           
           rdfs:comment "This class represent a parameter of a process template. A Parameter must be an Input or an Output (or both). A parameter is both an Input and Output when it is used on both sides of a nested workflow."@en .



###  http://www.wf4ever-project.org/vocab/wf#ProcessTemplate

:ProcessTemplate rdf:type owl:Class ;
                 
                 rdfs:comment """A process template is used to describe a class of actions that when enacted give rise to processes. A process template can have 0 or more Parameter associated using hasInput and hasOutput, signifying what kind of parameters the process will require and return.
"""@en .



###  http://www.wf4ever-project.org/vocab/wf#WorkflowTemplate

:WorkflowTemplate rdf:type owl:Class ;
                  
                  rdfs:subClassOf :ProcessTemplate ;
                  
                  rdfs:comment """A workflow template is a directed graph in which the nodes are process templates and the edges represent data dependencies between the constituent process templates.

A WorkflowTemplate defines associated Process Templates using hasProcessTemplate. A specialisation of this property is hasSubWorkflowTemplate, signifying that the process is a WorkflowTemplate itself, which is further described in a similar fashion.

As a subclass of ProcessTemplate a WorkflowTemplate can also define hasInput/hasOutput Parameters. 

Parameters are linked using DataLink instances associated with the WorkflowTemplate using hasDataLink.

A Parameter defined with hasInput on a WorkflowTemplate is considered an Input \"outside\" the workflow template (ie. if it is a subworkflow), but an Output \"inside\" the workflow template. Thus such Parameters can be linked \"through\" the workflow template.


Example:
##
@prefix wf: <http://www.wf4ever-project.org/vocab/wf#> .
:outerWorkflow a wf:WorkflowTemplate ;
  wf:hasSubWorkflowTemplate :innerWorkflow ;
  wf:hasProcessTemplate :procA, :procC .

:procA a wf:ProcessTemplate ;
  wf:hasOutput :param1 .

:procC a wf:ProcessTemplate ;
  wf:hasInput :param2 ;
  wf:hasOutput :param3 .


:innerWorkflow a wf:WorkflowTemplate ;
  wf:hasInput :param4 ;
  wf:hasOutput :param5 ;
  wf:hasProcessTemplate :procB .

:procB a wf:ProcessTemplate ;
  wf:hasInput :param6 ;
  wf:hasOutput :param7 .

:innerWorkflow wf:hasDataLink 
   [ wf:hasSource :param4; wf:hasSink :param6 ], 
   [ wf:hasSource :param7; wf:hasSink :param5 ] .

:outerWorkflow wf:hasDataLink
  [ wf:hasSource :param1; wf:hasSink :param4 ],
  [ wf:hasSource :param5; wf:hasSink :param2 ] .

##


In this example :param1 is the output of :procA. :param1 is the source in a datalink that goes to the input :param4 of the :innerWorkflow. :param4 is however also the source of an inner datalink, going to input :param6 of the nested :procB.

From this :param4 is both an wf:Input and wf:Output (which is why these two classes are not disjoint)"""@en .




###  Generated by the OWL API (version 3.2.3.1824) http://owlapi.sourceforge.net

